Clean and simplify some code

src/Experiments/SimplyTypedArithmetic.v
@@ -10,6 +10,7 @@ Require Import Crypto.Util.ListUtil Coq.Lists.List Crypto.Util.NatUtil.
 Require Import QArith.QArith_base QArith.Qround Crypto.Util.QUtil.
 Require Import Crypto.Algebra.Ring Crypto.Util.Decidable.Bool2Prop.
 Require Import Crypto.Algebra.Ring.
+Require Import Crypto.Algebra.SubsetoidRing.
 Require Import Crypto.Arithmetic.PrimeFieldTheorems.
 Require Import Crypto.Util.ZUtil.Tactics.PullPush.Modulo.
 Require Import Crypto.Util.ZRange.
@@ -25,6 +26,7 @@ Require Import Crypto.Util.ZUtil.AddGetCarry Crypto.Util.ZUtil.MulSplit.
 Require Import Crypto.Util.ZUtil.Tactics.LtbToLt.
 Require Import Crypto.Util.ZUtil.Tactics.PullPush.Modulo.
 Require Import Crypto.Util.Tactics.SpecializeBy.
+Require Import Crypto.Util.Tactics.SplitInContext.
 Require Import Crypto.Util.Notations.
 Require Import Crypto.Util.ZUtil.Definitions.
 Import ListNotations. Local Open Scope Z_scope.
@@ -1032,6 +1034,13 @@ Module Ring.
   Local Notation is_bounded_by2 bounds ls
     := (let '(a, b) := ls in andb (is_bounded_by bounds a) (is_bounded_by bounds b)).
 
+  Lemma length_is_bounded_by bounds ls
+    : is_bounded_by bounds ls = true -> length ls = length bounds.
+  Proof.
+    intro H.
+    apply fold_andb_map_length in H; congruence.
+  Qed.
+
   Section ring_goal.
     Context (weight : nat -> Z)
             (weight_0 : weight 0%nat = 1)
@@ -1134,221 +1143,35 @@ Module Ring.
                 -> is_bounded_by tight_bounds (Interp_rencodev arg) = true
                    /\ Interp_rencodev arg = encodemod arg).
 
-    Definition encodedT
-      := { ls : list Z | is_bounded_by tight_bounds ls = true }.
+    Local Notation T := (list Z) (only parsing).
+    Local Notation encoded_ok ls
+      := (is_bounded_by tight_bounds ls = true) (only parsing).
+    Local Notation encoded_okf := (fun ls => encoded_ok ls) (only parsing).
 
-    Definition list_of_encodedT (v : encodedT) : list _
-      := proj1_sig v.
-
-    Lemma length_list_of_encodedT v : List.length (list_of_encodedT v) = n.
-    Proof.
-      destruct v as [v H]; cbn in H |- *.
-      apply fold_andb_map_length in H; rewrite <- H.
-      assumption.
-    Qed.
-
-    Definition Zdecode (v : encodedT)
-      := list_of_encodedT v.
-    Definition Fdecode (v : encodedT) : F m
-      := F.of_Z m (Positional.eval weight n (Zdecode v)).
-    Definition encodedT_eq (x y : encodedT)
+    Definition Fdecode (v : T) : F m
+      := F.of_Z m (Positional.eval weight n v).
+    Definition T_eq (x y : T)
       := Fdecode x = Fdecode y.
 
-    Lemma length_Zdecode v : List.length (Zdecode v) = n.
-    Proof. apply length_list_of_encodedT. Qed.
+    Definition encodedT := sig encoded_okf.
 
-
-    Local Ltac specialize_from_interp _ :=
-      repeat match goal with
-             | [ H := ?Interp_rv ?arg, Hc : context[?Interp_rv] |- _ ]
-               => unique pose proof (Hc arg)
-             end.
-    Local Ltac specialize_with_bounded _ :=
-      repeat match goal with
-             | _ => progress cbv [Zdecode list_of_encodedT] in *
-             | _ => progress cbn [proj1_sig fst snd] in *
-             | [ H : context[andb ?x ?y = true] |- _ ]
-               => rewrite (Bool.andb_true_iff x y) in H
-             | [ H : _ /\ _ -> _ |- _ ] => specialize (fun a b => H (conj a b))
-             | _ => progress destruct_head'_and
-             | [ H : ?f (proj1_sig ?v) = true -> _ |- _ ]
-               => specialize (H (proj2_sig v)); hnf in H
-             | [ H : ?x = true -> _, H' : ?x = true |- _ ]
-               => specialize (H H'); hnf in H
-             | [ H : ?x = true |- { pf : ?x = true | _ } ] => exists H
-             end.
-    Local Ltac rewrite_interp _ :=
-      repeat match goal with
-             | [ H := _ |- _ ] => subst H
-             | [ H : ?x = _ |- context[?x] ] => rewrite H
-             | _ => rewrite expanding_id_id
-             | [ |- ?x = ?x ] => reflexivity
-             | [ |- List.length (proj1_sig _) = _ ] => apply length_list_of_encodedT
-             end.
-
-    Local Ltac solve_encodedT _ :=
-      specialize_from_interp ();
-      specialize_with_bounded ();
-      rewrite_interp ().
-
-    Definition ring_mul_sig
-      : forall (x y : encodedT),
-        { v : encodedT
-        | Zdecode v = carry_mulmod (Zdecode x, Zdecode y) }.
-    Proof.
-      simple refine
-             (fun x y
-              => let x' := Interp_rrelaxv (proj1_sig x) in
-                 let y' := Interp_rrelaxv (proj1_sig y) in
-                 let v' := Interp_rcarry_mulv (x', y') in
-                 let pf : { pf0 : _ | Zdecode (exist _ v' pf0) = _ }
-                     := _ in
-                 exist _ (exist _ v' (proj1_sig pf)) (proj2_sig pf)).
-      clear dependent HInterp_rzerov; clear dependent HInterp_ronev.
-      abstract solve_encodedT ().
-    Defined.
-
-    Definition ring_add_sig
-      : forall (x y : encodedT),
-        { v : encodedT
-        | Zdecode v = carrymod (addmod (Zdecode x, Zdecode y)) }.
-    Proof.
-      simple refine
-             (fun x y
-              => let v'' := Interp_raddv (proj1_sig x, proj1_sig y) in
-                 let v' := Interp_rcarryv v'' in
-                 let pf : { pf0 : _ | Zdecode (exist _ v' pf0) = _ }
-                     := _ in
-                 exist _ (exist _ v' (proj1_sig pf)) (proj2_sig pf)).
-      clear dependent HInterp_rzerov; clear dependent HInterp_ronev.
-      abstract solve_encodedT ().
-    Defined.
-    Definition ring_sub_sig
-      : forall (x y : encodedT),
-        { v : encodedT
-        | Zdecode v = carrymod (submod (Zdecode x, Zdecode y)) }.
-    Proof.
-      simple refine
-             (fun x y
-              => let v'' := Interp_rsubv (proj1_sig x, proj1_sig y) in
-                 let v' := Interp_rcarryv v'' in
-                 let pf : { pf0 : _ | Zdecode (exist _ v' pf0) = _ }
-                     := _ in
-                 exist _ (exist _ v' (proj1_sig pf)) (proj2_sig pf)).
-      clear dependent HInterp_rzerov; clear dependent HInterp_ronev.
-      abstract solve_encodedT ().
-    Defined.
-    Definition ring_opp_sig
-      : forall (x : encodedT),
-        { v : encodedT
-        | Zdecode v = carrymod (oppmod (Zdecode x)) }.
-    Proof.
-      simple refine
-             (fun x
-              => let v'' := Interp_roppv (proj1_sig x) in
-                 let v' := Interp_rcarryv v'' in
-                 let pf : { pf0 : _ | Zdecode (exist _ v' pf0) = _ }
-                     := _ in
-                 exist _ (exist _ v' (proj1_sig pf)) (proj2_sig pf)).
-      clear dependent HInterp_rzerov; clear dependent HInterp_ronev.
-      abstract solve_encodedT ().
-    Defined.
-    Definition ring_zero_sig
-      : { v : encodedT
-        | Zdecode v = zeromod }.
-    Proof.
-      simple refine
-             (let v' := Interp_rzerov in
-              let pf : { pf0 : _ | Zdecode (exist _ v' pf0) = _ }
-                  := _ in
-              exist _ (exist _ v' (proj1_sig pf)) (proj2_sig pf)).
-      cbn; clear -HInterp_rzerov.
-      abstract (destruct HInterp_rzerov; constructor; assumption).
-    Defined.
-    Definition ring_one_sig
-      : { v : encodedT
-        | Zdecode v = onemod }.
-    Proof.
-      simple refine
-             (let v' := Interp_ronev in
-              let pf : { pf0 : _ | Zdecode (exist _ v' pf0) = _ }
-                  := _ in
-              exist _ (exist _ v' (proj1_sig pf)) (proj2_sig pf)).
-      cbn; clear -HInterp_ronev.
-      abstract (destruct HInterp_ronev; cbn; constructor; assumption).
-    Defined.
-    Arguments Z.mul !_ !_ .
-    Definition ring_encode_sig
-      : forall (x : F m),
-        { v : encodedT
-        | Zdecode v = encodemod (F.to_Z x) }.
-    Proof.
-      simple refine
-             (fun v
-              => let pf1 := _ in
-                 let arg := F.to_Z v in
-                 let Hrencodev' := HInterp_rencodev arg pf1 in
-                 let v' := Interp_rencodev arg in
-                 let pf : { pf0 : _ | Zdecode (exist _ v' pf0) = _ }
-                     := _ in
-                 exist _ (exist _ v' (proj1_sig pf)) (proj2_sig pf)).
-      { generalize m_eq.
-        generalize sc_pos.
-        cbn; clear -v.
-        abstract (
-            intros sc_pos m_eq;
-            destruct v as [v Hv]; cbn; rewrite m_eq in Hv;
-            pose proof (Z.mod_pos_bound v _ sc_pos);
-            rewrite Bool.andb_true_iff; split; Z.ltb_to_lt; lia
-          ). }
-      { cbv [Zdecode list_of_encodedT]; cbn [proj1_sig].
-        subst v' arg; clearbody Hrencodev'; cbv beta zeta in *.
-        clear -Hrencodev'.
-        abstract (constructor; apply Hrencodev'). }
-    Defined.
-
-    Lemma length_addmod x y
-      : List.length (addmod (Zdecode x, Zdecode y)) = n.
-    Proof.
-      destruct (HInterp_raddv (Zdecode x, Zdecode y)) as [H0 H1];
-        [ .. | apply fold_andb_map_length in H0; rewrite <- H1, <- H0; assumption ].
-      cbv [Zdecode fst snd list_of_encodedT].
-      rewrite (proj2_sig x), (proj2_sig y); reflexivity.
-    Qed.
-    Lemma length_submod x y
-      : List.length (submod (Zdecode x, Zdecode y)) = n.
-    Proof.
-      destruct (HInterp_rsubv (Zdecode x, Zdecode y)) as [H0 H1];
-        [ .. | apply fold_andb_map_length in H0; rewrite <- H1, <- H0; assumption ].
-      cbv [Zdecode fst snd list_of_encodedT].
-      rewrite (proj2_sig x), (proj2_sig y); reflexivity.
-    Qed.
-    Lemma length_oppmod x
-      : List.length (oppmod (Zdecode x)) = n.
-    Proof.
-      destruct (HInterp_roppv (Zdecode x)) as [H0 H1];
-        [ .. | apply fold_andb_map_length in H0; rewrite <- H1, <- H0; assumption ].
-      cbv [Zdecode fst snd list_of_encodedT].
-      rewrite (proj2_sig x); reflexivity.
-    Qed.
-
-    Definition ring_mul x y := proj1_sig (ring_mul_sig x y).
-    Definition ring_add x y := proj1_sig (ring_add_sig x y).
-    Definition ring_sub x y := proj1_sig (ring_sub_sig x y).
-    Definition ring_opp x := proj1_sig (ring_opp_sig x).
-    Definition ring_zero := proj1_sig ring_zero_sig.
-    Definition ring_one := proj1_sig ring_one_sig.
-    Definition ring_encode x := proj1_sig (ring_encode_sig x).
+    Definition ring_mul (x y : T) : T
+      := Interp_rcarry_mulv (Interp_rrelaxv x, Interp_rrelaxv y).
+    Definition ring_add (x y : T) : T := Interp_rcarryv (Interp_raddv (x, y)).
+    Definition ring_sub (x y : T) : T := Interp_rcarryv (Interp_rsubv (x, y)).
+    Definition ring_opp (x : T) : T := Interp_rcarryv (Interp_roppv x).
+    Definition ring_encode (x : F m) : T := Interp_rencodev (F.to_Z x).
 
     Definition GoodT : Prop
-      := @Hierarchy.ring
-           encodedT encodedT_eq ring_zero ring_one ring_opp ring_add ring_sub ring_mul
-         /\ @Ring.is_homomorphism
-              (F m) eq 1%F F.add F.mul
-              encodedT encodedT_eq ring_one ring_add ring_mul ring_encode
-         /\ @Ring.is_homomorphism
-              encodedT encodedT_eq ring_one ring_add ring_mul
-              (F m) eq 1%F F.add F.mul
+      := @subsetoid_ring
+           (list Z) encoded_okf T_eq
+           Interp_rzerov Interp_ronev ring_opp ring_add ring_sub ring_mul
+         /\ @is_subsetoid_homomorphism
+              (F m) (fun _ => True) eq 1%F F.add F.mul
+              (list Z) encoded_okf T_eq Interp_ronev ring_add ring_mul ring_encode
+         /\ @is_subsetoid_homomorphism
+              (list Z) encoded_okf T_eq Interp_ronev ring_add ring_mul
+              (F m) (fun _ => True) eq 1%F F.add F.mul
               Fdecode.
 
     Hint Rewrite ->@F.to_Z_add : push_FtoZ.
@@ -1356,41 +1179,46 @@ Module Ring.
     Hint Rewrite ->@F.to_Z_opp : push_FtoZ.
     Hint Rewrite ->@F.to_Z_of_Z : push_FtoZ.
 
-    Local Ltac rewrite_proj2_sig _ :=
-      lazymatch goal with
-      | [ |- context[proj1_sig ?x] ] => rewrite (proj2_sig x)
-      end.
+    Lemma Fm_bounded_alt (x : F m)
+      : (0 <=? F.to_Z x) && (F.to_Z x <=? 'm - 1) = true.
+    Proof using m_eq.
+      clear -m_eq.
+      destruct x as [x H]; cbn [F.to_Z proj1_sig].
+      pose proof (Z.mod_pos_bound x ('m)).
+      rewrite andb_true_iff; split; Z.ltb_to_lt; lia.
+    Qed.
 
     Lemma Good : GoodT.
     Proof.
-      eapply ring_by_isomorphism; intros; [ | reflexivity | .. ]; rewrite F.eq_to_Z_iff;
-        cbv [F.sub Fdecode];
-        autorewrite with push_FtoZ;
-        pull_Zmod;
-        rewrite ?Z.add_opp_r.
-      { cbv [ring_encode]; rewrite_proj2_sig ().
-        erewrite m_eq, Hencodemod, <- m_eq by assumption.
-        let A := lazymatch goal with A : F _ |- _ => A end in
-        destruct A as [v Hv]; cbn; congruence. }
-      { cbv [ring_zero]; rewrite_proj2_sig ().
-        erewrite m_eq, Hzeromod, Zmod_0_l by eassumption; reflexivity. }
-      { cbv [ring_one]; rewrite_proj2_sig ().
-        cbn; erewrite m_eq, Honemod; reflexivity. }
-      { cbv [ring_opp]; rewrite_proj2_sig ().
-        erewrite m_eq, Hcarrymod, Hoppmod
-          by eauto using length_Zdecode, length_oppmod;
-          reflexivity. }
-      { cbv [ring_add]; rewrite_proj2_sig ().
-        erewrite m_eq, Hcarrymod, Haddmod
-          by eauto using length_Zdecode, length_addmod;
-          reflexivity. }
-      { cbv [ring_sub]; rewrite_proj2_sig ().
-        erewrite m_eq, Hcarrymod, Hsubmod
-          by eauto using length_Zdecode, length_submod;
-          reflexivity. }
-      { cbv [ring_mul]; rewrite_proj2_sig ().
-        erewrite m_eq, Hcarry_mulmod
-          by eauto using length_Zdecode; reflexivity. }
+      split_and.
+      eapply subsetoid_ring_by_ring_isomorphism;
+        cbv [ring_opp ring_add ring_sub ring_mul ring_encode F.sub] in *;
+        repeat match goal with
+               | _ => solve [ auto using andb_true_intro, conj with nocore ]
+               | _ => progress intros
+               | _ => progress cbn [fst snd]
+               | [ H : _ |- is_bounded_by _ _ = true ] => apply H
+               | [ |- _ <-> _ ] => reflexivity
+               | [ |- _ = _ :> Z ] => first [ reflexivity | rewrite <- m_eq; reflexivity ]
+               | [ H : context[?x] |- Fdecode ?x = _ ] => rewrite H
+               | [ H : context[?x _] |- Fdecode (?x _) = _ ] => rewrite H
+               | _ => progress cbv [Fdecode]
+               | [ |- _ = _ :> F _ ] => apply F.eq_to_Z_iff
+               | _ => progress autorewrite with push_FtoZ
+               | _ => rewrite m_eq
+               | [ H : context[?x _] |- context[eval (?x _)] ] => rewrite H
+               | [ H : context[?x] |- context[eval ?x] ] => rewrite H
+               | [ |- context[List.length ?x] ]
+                 => erewrite (length_is_bounded_by _ x)
+                   by eauto using andb_true_intro, conj with nocore
+               | [ |- _ = _ :> Z ]
+                 => push_Zmod; reflexivity
+               | _ => pull_Zmod; rewrite Z.add_opp_r
+               | _ => rewrite expanding_id_id
+               | [ |- context[F.to_Z _ mod (_ - _)] ]
+                 => rewrite <- m_eq, F.mod_to_Z
+               | _ => rewrite <- m_eq; apply Fm_bounded_alt
+               end.
     Qed.
   End ring_goal.
 End Ring.
@@ -1487,19 +1315,25 @@ Module Compilers.
       | Pair {A B} (a : expr A) (b : expr B) : expr (A * B)
       | Abs {s d} (f : var s -> expr d) : expr (s -> d).
 
+      Definition Expr {ident : type -> type -> Type} t := forall var, @expr ident var t.
+
+      Definition APP {ident s d} (f : Expr (s -> d)) (x : Expr s) : Expr d
+        := fun var => @App ident var s d (f var) (x var).
+
       Module Export Notations.
         Bind Scope expr_scope with expr.
         Delimit Scope expr_scope with expr.
+        Bind Scope Expr_scope with Expr.
+        Delimit Scope Expr_scope with Expr.
 
         Infix "@" := App : expr_scope.
+        Infix "@" := APP : Expr_scope.
         Infix "@@" := AppIdent : expr_scope.
         Notation "( x , y , .. , z )" := (Pair .. (Pair x%expr y%expr) .. z%expr) : expr_scope.
         Notation "( )" := TT : expr_scope.
         Notation "()" := TT : expr_scope.
         Notation "'λ'  x .. y , t" := (Abs (fun x => .. (Abs (fun y => t%expr)) ..)) : expr_scope.
       End Notations.
-
-      Definition Expr {ident : type -> type -> Type} t := forall var, @expr ident var t.
 
       Section unexpr.
         Context {ident : type -> type -> Type}
@@ -1531,6 +1365,10 @@ Module Compilers.
              end.
 
         Definition Interp {t} (e : Expr t) := interp (e _).
+
+        Definition Interp_APP {s d} (f : @Expr ident (s -> d)) (x : @Expr ident s)
+          : Interp (f @ x)%Expr = Interp f (Interp x)
+          := eq_refl.
       End with_ident.
 
       Ltac require_primitive_const term :=
@@ -4891,6 +4729,7 @@ Module Compilers.
     Definition partial_reduce_with_bounds1 {s d} (e : @expr (partial.value var) (s -> d))
                (b : ZRange.type.interp s)
       := partial.expr.reify (@partial_reduce_with_bounds1' s d e b).
+
   End partial_reduce.
 
   Definition PartialReduce {t} (e : Expr t) : Expr t
@@ -5556,7 +5395,7 @@ Module Pipeline.
        end.
 
   Definition BoundsPipeline
-             (with_dead_code_elimination : bool := true)
+             (with_dead_code_elimination : bool)
              relax_zrange
              {s d}
              (E : Expr (s -> d))
@@ -5564,6 +5403,9 @@ Module Pipeline.
              out_bounds
   : ErrorT (Expr (s -> d))
     := let E := PartialReduce E in
+       (* Note that DCE evaluates the expr with two different [var]
+          arguments, and so will likely result in a pipeline that is
+          2x slower *)
        let E := if with_dead_code_elimination then DeadCodeElimination.EliminateDead E else E in
        let E := ReassociateSmallConstants.Reassociate (2^8) E in
        let E := CheckedPartialReduceWithBounds1 relax_zrange E arg_bounds out_bounds in
@@ -5574,7 +5416,7 @@ Module Pipeline.
        E.
 
   Lemma BoundsPipeline_correct
-             (*with_dead_code_elimination : bool*)
+             (with_dead_code_elimination : bool)
              relax_zrange
              (Hrelax : forall r r' z : zrange,
                  (z <=? r)%zrange = true -> relax_zrange r = Some r' -> (z <=? r')%zrange = true)
@@ -5583,13 +5425,13 @@ Module Pipeline.
              arg_bounds
              out_bounds
              rv
-             (Hrv : BoundsPipeline (*with_dead_code_elimination*) relax_zrange E arg_bounds out_bounds = Success rv)
+             (Hrv : BoundsPipeline with_dead_code_elimination relax_zrange E arg_bounds out_bounds = Success rv)
     : forall arg
              (Harg : ZRange.type.is_bounded_by arg_bounds arg = true),
       ZRange.type.is_bounded_by out_bounds (Interp rv arg) = true
       /\ Interp rv arg = Interp E arg.
   Proof.
-    cbv [BoundsPipeline] in *; edestruct (CheckedPartialReduceWithBounds1 _ _ _ _) eqn:H.
+    cbv [BoundsPipeline Let_In] in *; edestruct (CheckedPartialReduceWithBounds1 _ _ _ _) eqn:H.
     inversion Hrv; subst.
     { intros; eapply CheckedPartialReduceWithBounds1_Correct in H; [ | eassumption.. ].
       destruct H as [H0 H1].
@@ -5598,14 +5440,50 @@ Module Pipeline.
     { congruence. }
   Qed.
 
+  Definition BoundsPipeline_correct_transT
+             {s d}
+             (E : Expr (s -> d))
+             arg_bounds
+             out_bounds
+             (InterpE : type.interp s -> type.interp d)
+             (rv : Expr (s -> d))
+    := forall arg
+              (Harg : ZRange.type.is_bounded_by arg_bounds arg = true),
+      ZRange.type.is_bounded_by out_bounds (Interp rv arg) = true
+      /\ Interp rv arg = InterpE arg.
+
+  Lemma BoundsPipeline_correct_trans
+        (with_dead_code_elimination : bool)
+        relax_zrange
+        (Hrelax
+         : forall r r' z : zrange,
+            (z <=? r)%zrange = true -> relax_zrange r = Some r' -> (z <=? r')%zrange = true)
+        {s d}
+        (E : Expr (s -> d))
+        arg_bounds out_bounds
+        (InterpE : type.interp s -> type.interp d)
+        (InterpE_correct
+         : forall arg
+                  (Harg : ZRange.type.is_bounded_by arg_bounds arg = true),
+            Interp E arg = InterpE arg)
+        rv (Hrv : BoundsPipeline with_dead_code_elimination relax_zrange E arg_bounds out_bounds = Success rv)
+    : BoundsPipeline_correct_transT E arg_bounds out_bounds InterpE rv.
+  Proof.
+    intros arg Harg; rewrite <- InterpE_correct by assumption.
+    eapply @BoundsPipeline_correct; eassumption.
+  Qed.
+    
   Definition BoundsPipelineConst
-             (with_dead_code_elimination : bool := true)
+             (with_dead_code_elimination : bool)
              relax_zrange
              {t}
              (E : Expr t)
              bounds
   : ErrorT (Expr t)
     := let E := PartialReduce E in
+       (* Note that DCE evaluates the expr with two different [var]
+          arguments, and so will likely result in a pipeline that is
+          2x slower *)
        let E := if with_dead_code_elimination then DeadCodeElimination.EliminateDead E else E in
        let E := ReassociateSmallConstants.Reassociate (2^8) E in
        let E := CheckedPartialReduceWithBounds0 relax_zrange E bounds in
@@ -5616,7 +5494,7 @@ Module Pipeline.
        E.
 
   Lemma BoundsPipelineConst_correct
-             (*with_dead_code_elimination : bool*)
+             (with_dead_code_elimination : bool)
              relax_zrange
              (Hrelax : forall r r' z : zrange,
                  (z <=? r)%zrange = true -> relax_zrange r = Some r' -> (z <=? r')%zrange = true)
@@ -5624,17 +5502,45 @@ Module Pipeline.
              (E : Expr d)
              bounds
              rv
-             (Hrv : BoundsPipelineConst (*with_dead_code_elimination*) relax_zrange E bounds = Success rv)
+             (Hrv : BoundsPipelineConst with_dead_code_elimination relax_zrange E bounds = Success rv)
     : ZRange.type.is_bounded_by bounds (Interp rv) = true
       /\ Interp rv = Interp E.
   Proof.
-    cbv [BoundsPipelineConst] in *; edestruct (CheckedPartialReduceWithBounds0 _ _ _) eqn:H.
+    cbv [BoundsPipelineConst Let_In] in *; edestruct (CheckedPartialReduceWithBounds0 _ _ _) eqn:H.
     inversion Hrv; subst.
     { intros; eapply CheckedPartialReduceWithBounds0_Correct in H; [ | eassumption.. ].
       destruct H as [H0 H1].
       split; [ exact H1 | rewrite H0 ].
       exact admit. (* interp correctness *) }
     { congruence. }
+  Qed.
+  
+  Definition BoundsPipelineConst_correct_transT
+             {t}
+             (E : Expr t)
+             out_bounds
+             (InterpE : type.interp t)
+             (rv : Expr t)
+    := ZRange.type.is_bounded_by out_bounds (Interp rv) = true
+       /\ Interp rv = InterpE.
+
+  Lemma BoundsPipelineConst_correct_trans
+        (with_dead_code_elimination : bool)
+        relax_zrange
+        (Hrelax
+         : forall r r' z : zrange,
+            (z <=? r)%zrange = true -> relax_zrange r = Some r' -> (z <=? r')%zrange = true)
+        {t}
+        (E : Expr t)
+        out_bounds
+        (InterpE : type.interp t)
+        (InterpE_correct : Interp E = InterpE)
+        rv
+        (Hrv : BoundsPipelineConst with_dead_code_elimination relax_zrange E out_bounds = Success rv)
+    : BoundsPipelineConst_correct_transT E out_bounds InterpE rv.
+  Proof.
+    rewrite <- InterpE_correct.
+    eapply @BoundsPipelineConst_correct; eassumption.
   Qed.
 End Pipeline.
 
@@ -5797,401 +5703,146 @@ Section rcarry_mul.
                            then Pipeline.Error (Pipeline.Value_not_lt "0 < machine_wordsize" 0 machine_wordsize)
                            else res.
 
-  Lemma check_args_success_id {T} {rv : T} {res}
-    : check_args res = Pipeline.Success rv
-      -> res = Pipeline.Success rv.
-  Proof.
-    cbv [check_args]; break_innermost_match; congruence.
-  Qed.
+  Local Ltac t_solve_interp :=
+    try solve [ reflexivity
+              | cbn -[reify_list];
+                try (rewrite interp_reify_list, map_map; cbn;
+                     erewrite map_ext with (g:=id), map_id; try reflexivity);
+                try (intros []; reflexivity) ].
+  Lemma Interp_rs : Interp rs = s. Proof. reflexivity. Qed.
+  Lemma Interp_rc : Interp rc = c. Proof. t_solve_interp. Qed.
+  Lemma Interp_rn : Interp rn = n. Proof. reflexivity. Qed.
+  Lemma Interp_ridxs : Interp ridxs = idxs. Proof. t_solve_interp. Qed.
 
-  Local Ltac solve_correct_gen pipeline_lem gen_correct :=
-    let Hrv := lazymatch goal with H : ?rop = Pipeline.Success _ |- _ => H end in
-    let rop := lazymatch type of Hrv with ?rop = Pipeline.Success _ => rop end in
-    hnf; intros; cbv [rop] in Hrv;
-    eapply pipeline_lem in Hrv; [ | eassumption.. ];
-    let Hrv' := fresh "Hrv'" in
-    destruct Hrv as [Hrv Hrv'];
-    apply conj; [ exact Hrv | rewrite Hrv' ];
-    repeat match goal with H := _ |- _ => subst H end;
-    erewrite <- gen_correct;
-    cbv [expr.Interp];
-    cbn [expr.interp];
-    f_equal;
-    cbn -[reify_list];
-    try (rewrite interp_reify_list, map_map; cbn;
-         erewrite map_ext with (g:=id), map_id; try reflexivity);
-    try (intros []; reflexivity).
-  Local Ltac solve_correct gen_correct :=
-    solve_correct_gen Pipeline.BoundsPipeline_correct gen_correct.
-  Local Ltac solve_correct_const gen_correct :=
-    solve_correct_gen Pipeline.BoundsPipelineConst_correct gen_correct.
+  Local Hint Rewrite @Interp_APP : interp_correct.
+  Local Hint Rewrite Interp_rs Interp_rc Interp_rn Interp_ridxs : interp_correct.
+  Local Hint Rewrite carry_mul_gen_correct carry_gen_correct id_gen_correct add_gen_correct sub_gen_correct opp_gen_correct encode_gen_correct zero_gen_correct one_gen_correct : interp_correct.
 
-  (* TODO(jgross): open bug about sensitivity of order of arguments on type inference with interp, expr *)
-  (* TODO(jgross): Make @ apply to Expr, not just expr *)
+  Local Ltac do_interp_correct :=
+    intros; repeat autorewrite with interp_correct; reflexivity.
+
+  Notation type_of := ((fun T (_ : T) => T) _).
+  Notation type_of_strip_arrow := ((fun s (d : Prop) (_ : s -> d) => d) _ _).
+
+  Notation BoundsPipeline rop in_bounds out_bounds
+    := (Pipeline.BoundsPipeline
+          false
+          relax_zrange
+          rop%Expr in_bounds out_bounds).
+
+  Notation BoundsPipelineConst rop out_bounds
+    := (Pipeline.BoundsPipelineConst
+          false
+          relax_zrange
+          rop%Expr out_bounds).
+
+  Notation BoundsPipeline_correct rop in_bounds out_bounds op
+    := (@Pipeline.BoundsPipeline_correct_trans
+          false
+          relax_zrange
+          relax_zrange_good
+          _ _
+          rop%Expr
+          in_bounds
+          out_bounds
+          op
+          ltac:(do_interp_correct)).
+
+  Notation BoundsPipelineConst_correct rop out_bounds op
+    := (@Pipeline.BoundsPipelineConst_correct_trans
+          false
+          relax_zrange
+          relax_zrange_good
+          _
+          rop%Expr
+          out_bounds
+          op
+          ltac:(do_interp_correct)).
+
+  (* N.B. We only need [rcarry_mul] if we want to extract the Pipeline; otherwise we can just use [rcarry_mul_correct] *)
   Definition rcarry_mul
-    := let res := Pipeline.BoundsPipeline
-                    relax_zrange
-                    (fun var
-                     => (carry_mul_gen _)
-                          @ (rw _)
-                          @ (rs _)
-                          @ (rc _)
-                          @ (rn _)
-                          @ (rlen_c _)
-                          @ (ridxs _)
-                          @ (rlen_idxs _)
-                    )%expr
-                    (loose_bounds, loose_bounds)
-                    tight_bounds in
-       res.
+    := BoundsPipeline
+         (carry_mul_gen
+            @ rw @ rs @ rc @ rn @ rlen_c @ ridxs @ rlen_idxs)
+         (loose_bounds, loose_bounds)
+         tight_bounds.
 
-  Definition rcarry_mul_correctT
-             (rv : Expr (type.list type.Z * type.list type.Z -> type.list type.Z))
-    := (forall
-           arg
-           (Harg : ZRange.type.is_bounded_by (t:=type.prod (type.list type.Z) (type.list type.Z))
-                                             (loose_bounds, loose_bounds) arg = true),
-           ZRange.type.is_bounded_by (t:=type.list type.Z)
-                                     tight_bounds
-                                     (Interp rv arg) = true /\
-           Interp rv arg =
-           carry_mulmod (Interp rw) s c n (Interp rlen_c)
-                        idxs (Interp rlen_idxs) arg).
-  Check (@Pipeline.BoundsPipeline_correct
-           relax_zrange
-           _
-           _ _
-       ).
+  Definition rcarry_mul_correct
+    := BoundsPipeline_correct
+         (carry_mul_gen
+            @ rw @ rs @ rc @ rn @ rlen_c @ ridxs @ rlen_idxs)%Expr
+         (loose_bounds, loose_bounds)
+         tight_bounds
+         (carry_mulmod (Interp rw) s c n (Interp rlen_c) idxs (Interp rlen_idxs)).
 
-    Lemma rcarry_mul_correct
-        rv (Hrv : rcarry_mul = Pipeline.Success rv)
-    : rcarry_mul_correctT rv.
-  Proof. solve_correct carry_mul_gen_correct. Qed.
+  Definition rcarry_correct
+    := BoundsPipeline_correct
+         (carry_gen
+            @ rw @ rs @ rc @ rn @ rlen_c @ ridxs @ rlen_idxs)%Expr
+         loose_bounds
+         tight_bounds
+         (carrymod (Interp rw) s c n (Interp rlen_c) idxs (Interp rlen_idxs)).
 
+  Definition rrelax_correct
+    := BoundsPipeline_correct
+         (id_gen @ rn)%Expr
+         tight_bounds
+         loose_bounds
+         (expanding_id n).
 
+  Definition radd_correct
+    := BoundsPipeline_correct
+         (add_gen @ rw @ rn)%Expr
+         (tight_bounds, tight_bounds)
+         loose_bounds
+         (addmod (Interp rw) n).
 
-  Let BoundsPipeline21 in_bounds out_bounds res
-    := let res := Pipeline.BoundsPipeline
-                    relax_zrange
-                    (s:=(type.list type.Z * type.list type.Z)%ctype)
-                    (d:=(type.list type.Z)%ctype)
-                    res
-                    (in_bounds, in_bounds)
-                    out_bounds in
-       res.
+  Definition rsub_correct
+    := BoundsPipeline_correct
+         (sub_gen @ rw @ rs @ rc @ rn @ rlen_c @ rcoef)%Expr
+         (tight_bounds, tight_bounds)
+         loose_bounds
+         (submod (Interp rw) s c n (Interp rlen_c) (Interp rcoef)).
 
-  Let BoundsPipeline11 in_bounds out_bounds res
-    := let res := Pipeline.BoundsPipeline
-                    relax_zrange
-                    (s:=(type.list type.Z)%ctype)
-                    (d:=(type.list type.Z)%ctype)
-                    res
-                    (in_bounds)
-                    out_bounds in
-       res.
+  Definition ropp_correct
+    := BoundsPipeline_correct
+         (opp_gen @ rw @ rs @ rc @ rn @ rlen_c @ rcoef)%Expr
+         tight_bounds
+         loose_bounds
+         (oppmod (Interp rw) s c n (Interp rlen_c) (Interp rcoef)).
 
-  Definition rexpr_1_correctT_Interp
-             {t}
-             t_out
-             (Interp : Expr t -> _)
-             out_bounds
-             (f : type.interp t_out)
-             rv
-    := (ZRange.type.is_bounded_by out_bounds (Interp rv) = true
-        /\ Interp rv = f).
+  Definition rencode_correct
+    := BoundsPipeline_correct
+         (encode_gen @ rw @ rs @ rc @ rn @ rlen_c)%Expr
+         prime_bound
+         tight_bounds
+         (encodemod (Interp rw) s c n (Interp rlen_c)).
 
-  Definition rexpr_n1_correctT
-             t_in t_out
-             in_bounds out_bounds
-             (f : type.interp t_in -> type.interp t_out)
-             rv
-    := forall arg
-              (Harg : ZRange.type.is_bounded_by in_bounds arg = true),
-      @rexpr_1_correctT_Interp (t_in -> t_out) t_out (fun rv => Interp rv arg) out_bounds (f arg) rv.
+  Definition rzero_correct
+    := BoundsPipelineConst_correct
+         (zero_gen @ rw @ rs @ rc @ rn @ rlen_c)%Expr
+         tight_bounds
+         (zeromod (Interp rw) s c n (Interp rlen_c)).
 
-  Definition rexpr_1_correctT
-             t_out
-             out_bounds
-             (f : type.interp t_out)
-             rv
-    := @rexpr_1_correctT_Interp t_out t_out Interp out_bounds f rv.
+  Definition rone_correct
+    := BoundsPipelineConst_correct
+         (one_gen @ rw @ rs @ rc @ rn @ rlen_c)%Expr
+         tight_bounds
+         (onemod (Interp rw) s c n (Interp rlen_c)).
 
-  Definition rexpr_21_correctT
-             in_bounds out_bounds
-             (f : _ -> type.interp (type.list type.Z))
-             rv
-    := @rexpr_n1_correctT (type.list type.Z * type.list type.Z)
-                          (type.list type.Z)
-                          (in_bounds, in_bounds) out_bounds f rv.
-
-  Definition rexpr_11_correctT
-             in_bounds out_bounds
-             (f : _ -> type.interp (type.list type.Z))
-             rv
-    := @rexpr_n1_correctT (type.list type.Z)
-                          (type.list type.Z)
-                          in_bounds out_bounds f rv.
-
-  Definition rexpr_Z1_correctT
-             in_bounds out_bounds
-             (f : _ -> type.interp (type.list type.Z))
-             rv
-    := @rexpr_n1_correctT type.Z (type.list type.Z)
-                          in_bounds out_bounds f rv.
-
-  Definition rexpr_01_correctT
-             out_bounds
-             (f : type.interp (type.list type.Z))
-             rv
-    := @rexpr_1_correctT (type.list type.Z) out_bounds f rv.
-
-  Definition rcarry_mul_correctT
-             rv
-    := Eval hnf in
-        rexpr_21_correctT
-          loose_bounds tight_bounds
-          (carry_mulmod (Interp rw) s c n (Interp rlen_c) idxs (Interp rlen_idxs))
-          rv.
-  Eval cbv [rcarry_mul_correctT rexpr_1_correctT_Interp] in rcarry_mul_correctT.
-  Print rcarry_mul_correctT.
-
-  Lemma rcarry_mul_correct
-        rv (Hrv : rcarry_mul = Pipeline.Success rv)
-    : rcarry_mul_correctT rv.
-  Proof. solve_correct carry_mul_gen_correct. Qed.
-
-  Definition rcarry
-    := let res := Pipeline.BoundsPipeline
-                    false
-                    relax_zrange
-                    (s:=(type.list type.Z)%ctype)
-                    (d:=(type.list type.Z)%ctype)
-                    loose_bounds
-                    tight_bounds
-                    (fun var
-                     => (carry_gen _)
-                          @ (rw _)
-                          @ (rs _)
-                          @ (rc _)
-                          @ (rn _)
-                          @ (rlen_c _)
-                          @ (ridxs _)
-                          @ (rlen_idxs _)
-                    )%expr in
-       res.
-
-  Definition rcarry_correctT
-             rv
-    := Eval hnf in
-        rexpr_11_correctT
-          loose_bounds tight_bounds
-          (carrymod (Interp rw) s c n (Interp rlen_c) idxs (Interp rlen_idxs))
-          rv.
-
-  Lemma rcarry_correct
-        rv (Hrv : rcarry = Pipeline.Success rv)
-    : rcarry_correctT rv.
-  Proof. solve_correct carry_gen_correct. Qed.
-
-  Definition rrelax
-    := let res := Pipeline.BoundsPipeline
-                    false
-                    relax_zrange
-                    (s:=(type.list type.Z)%ctype)
-                    (d:=(type.list type.Z)%ctype)
-                    tight_bounds
-                    loose_bounds
-                    (fun var
-                     => (id_gen _)
-                          @ (rn _)
-                    )%expr in
-       res.
-
-  Definition rrelax_correctT
-             rv
-    := Eval hnf in
-        rexpr_11_correctT
-          tight_bounds loose_bounds
-          (expanding_id n)
-          rv.
-
-  Lemma rrelax_correct
-        rv (Hrv : rrelax = Pipeline.Success rv)
-    : rrelax_correctT rv.
-  Proof. solve_correct id_gen_correct. Qed.
-
-  Definition radd
-    := let res := BoundsPipeline21
-                    tight_bounds
-                    loose_bounds
-                    (fun var
-                     => (add_gen _)
-                          @ (rw _)
-                          @ (rn _)
-                    )%expr in
-       res.
-
-  Definition radd_correctT
-             rv
-    := Eval hnf in
-        rexpr_21_correctT
-          tight_bounds loose_bounds
-          (addmod (Interp rw) n)
-          rv.
-
-  Lemma radd_correct
-        rv (Hrv : radd = Pipeline.Success rv)
-    : radd_correctT rv.
-  Proof. solve_correct add_gen_correct. Qed.
-
-  Definition rsub
-    := let res := BoundsPipeline21
-                    tight_bounds
-                    loose_bounds
-                    (fun var
-                     => (sub_gen _)
-                          @ (rw _)
-                          @ (rs _)
-                          @ (rc _)
-                          @ (rn _)
-                          @ (rlen_c _)
-                          @ (rcoef _)
-                    )%expr in
-       res.
-
-  Definition rsub_correctT
-             rv
-    := Eval hnf in
-        rexpr_21_correctT
-          tight_bounds loose_bounds
-          (submod (Interp rw) s c n (Interp rlen_c) (Interp rcoef))
-          rv.
-
-  Lemma rsub_correct
-        rv (Hrv : rsub = Pipeline.Success rv)
-    : rsub_correctT rv.
-  Proof. solve_correct sub_gen_correct. Qed.
-
-  Definition ropp
-    := let res := BoundsPipeline11
-                    tight_bounds
-                    loose_bounds
-                    (fun var
-                     => (opp_gen _)
-                          @ (rw _)
-                          @ (rs _)
-                          @ (rc _)
-                          @ (rn _)
-                          @ (rlen_c _)
-                          @ (rcoef _)
-                    )%expr in
-       res.
-
-  Definition ropp_correctT
-             rv
-    := Eval hnf in
-        rexpr_11_correctT
-          tight_bounds loose_bounds
-          (oppmod (Interp rw) s c n (Interp rlen_c) (Interp rcoef))
-          rv.
-
-  Lemma ropp_correct
-        rv (Hrv : ropp = Pipeline.Success rv)
-    : ropp_correctT rv.
-  Proof. solve_correct opp_gen_correct. Qed.
-
-  Definition rencode
-    := let res := Pipeline.BoundsPipeline
-                    false
-                    relax_zrange
-                    (s:=type.Z)
-                    (d:=(type.list type.Z)%ctype)
-                    (prime_bound)
-                    tight_bounds
-                    (fun var
-                     => (encode_gen _)
-                          @ (rw _)
-                          @ (rs _)
-                          @ (rc _)
-                          @ (rn _)
-                          @ (rlen_c _)
-                    )%expr in
-       res.
-
-  Definition rencode_correctT
-             rv
-    := Eval hnf in
-        rexpr_Z1_correctT
-          prime_bound tight_bounds
-          (encodemod (Interp rw) s c n (Interp rlen_c))
-          rv.
-
-  Lemma rencode_correct
-        rv (Hrv : rencode = Pipeline.Success rv)
-    : rencode_correctT rv.
-  Proof. solve_correct encode_gen_correct. Qed.
-
-  Definition rzero
-    := let res := Pipeline.BoundsPipelineConst
-                    false
-                    relax_zrange
-                    (t:=(type.list type.Z)%ctype)
-                    tight_bounds
-                    (fun var
-                     => (zero_gen _)
-                          @ (rw _)
-                          @ (rs _)
-                          @ (rc _)
-                          @ (rn _)
-                          @ (rlen_c _)
-                    )%expr in
-       res.
-
-  Definition rzero_correctT
-             rv
-    := Eval hnf in
-        rexpr_01_correctT
-          tight_bounds
-          (zeromod (Interp rw) s c n (Interp rlen_c))
-          rv.
-
-  Lemma rzero_correct
-        rv (Hrv : rzero = Pipeline.Success rv)
-    : rzero_correctT rv.
-  Proof. solve_correct_const zero_gen_correct. Qed.
-
-  Definition rone
-    := let res := Pipeline.BoundsPipelineConst
-                    false
-                    relax_zrange
-                    (t:=(type.list type.Z)%ctype)
-                    tight_bounds
-                    (fun var
-                     => (one_gen _)
-                          @ (rw _)
-                          @ (rs _)
-                          @ (rc _)
-                          @ (rn _)
-                          @ (rlen_c _)
-                    )%expr in
-       res.
-
-  Definition rone_correctT
-             rv
-    := Eval hnf in
-        rexpr_01_correctT
-          tight_bounds
-          (onemod (Interp rw) s c n (Interp rlen_c))
-          rv.
-
-  Lemma rone_correct
-        rv (Hrv : rone = Pipeline.Success rv)
-    : rone_correctT rv.
-  Proof. solve_correct_const one_gen_correct. Qed.
-
-  Let m : positive := Z.to_pos (s - Associational.eval c).
+  (* we need to strip off [Hrv : ... = Pipeline.Success rv] *)
+  Definition rcarry_mul_correctT rv : Prop := type_of_strip_arrow (@rcarry_mul_correct rv).
+  Definition rcarry_correctT rv : Prop := type_of_strip_arrow (@rcarry_correct rv).
+  Definition rrelax_correctT rv : Prop := type_of_strip_arrow (@rrelax_correct rv).
+  Definition radd_correctT rv : Prop := type_of_strip_arrow (@radd_correct rv).
+  Definition rsub_correctT rv : Prop := type_of_strip_arrow (@rsub_correct rv).
+  Definition ropp_correctT rv : Prop := type_of_strip_arrow (@ropp_correct rv).
+  Definition rencode_correctT rv : Prop := type_of_strip_arrow (@rencode_correct rv).
+  Definition rzero_correctT rv : Prop := type_of_strip_arrow (@rzero_correct rv).
+  Definition rone_correctT rv : Prop := type_of_strip_arrow (@rone_correct rv).
 
   Section make_ring.
+    Let m : positive := Z.to_pos (s - Associational.eval c).
     Context (curve_good : check_args (Pipeline.Success tt) = Pipeline.Success tt)
             {rcarry_mulv} (Hrmulv : rcarry_mul_correctT rcarry_mulv)
             {rcarryv} (Hrcarryv : rcarry_correctT rcarryv)
@@ -6284,40 +5935,29 @@ Section rcarry_mul.
            (Interp rw)
            n s c
            tight_bounds
-           length_tight_bounds
-           loose_bounds
-           m_eq
-           sc_pos
-           (Interp rrelaxv) Hrrelaxv
-           (carry_mulmod (Interp rw) s c n (Interp rlen_c) idxs (Interp rlen_idxs))
-           (Interp rcarry_mulv) Hrmulv
-           (carrymod (Interp rw) s c n (Interp rlen_c) idxs (Interp rlen_idxs))
-           (Interp rcarryv) Hrcarryv
-           (addmod (Interp rw) n)
-           (Interp raddv) Hraddv
-           (submod (Interp rw) s c n (Interp rlen_c) (Interp rcoef))
-           (Interp rsubv) Hrsubv
-           (oppmod (Interp rw) s c n (Interp rlen_c) (Interp rcoef))
-           (Interp roppv) Hroppv
-           (zeromod (Interp rw) s c n (Interp rlen_c))
-           (Interp rzerov) Hrzerov
-           (onemod (Interp rw) s c n (Interp rlen_c))
-           (Interp ronev) Hronev
-           (encodemod (Interp rw) s c n (Interp rlen_c))
-           (Interp rencodev) Hrencodev.
+           (Interp rrelaxv)
+           (Interp rcarry_mulv)
+           (Interp rcarryv)
+           (Interp raddv)
+           (Interp rsubv)
+           (Interp roppv)
+           (Interp rzerov)
+           (Interp ronev)
+           (Interp rencodev).
 
     Theorem Good : GoodT.
     Proof.
       pose proof use_curve_good; destruct_head'_and.
-      apply Ring.Good;
+      eapply Ring.Good;
         repeat first [ assumption
+                     | intros; apply eval_carry_mulmod
+                     | intros; apply eval_carrymod
+                     | intros; apply eval_addmod
+                     | intros; apply eval_submod
+                     | intros; apply eval_oppmod
+                     | intros; apply eval_encodemod
+                     | eassumption
                      | progress intros
-                     | rewrite eval_carry_mulmod
-                     | rewrite eval_carrymod
-                     | rewrite eval_addmod
-                     | rewrite eval_submod
-                     | rewrite eval_oppmod
-                     | rewrite eval_encodemod
                      | progress cbv [onemod zeromod]
                      | match goal with
                        | [ |- ?x = ?x ] => reflexivity
@@ -6487,39 +6127,39 @@ Module X25519_64.
   Definition machine_wordsize := 64.
 
   Derive base_51_relax
-         SuchThat (rrelax_correctT n s c base_51_relax)
+         SuchThat (rrelax_correctT n s c machine_wordsize base_51_relax)
          As base_51_relax_correct.
   Proof. Time solve_rrelax machine_wordsize. Time Qed.
   Derive base_51_carry_mul
-         SuchThat (rcarry_mul_correctT n s c base_51_carry_mul)
+         SuchThat (rcarry_mul_correctT n s c machine_wordsize base_51_carry_mul)
          As base_51_carry_mul_correct.
   Proof. Time solve_rcarry_mul machine_wordsize. Time Qed.
   Derive base_51_carry
-         SuchThat (rcarry_correctT n s c base_51_carry)
+         SuchThat (rcarry_correctT n s c machine_wordsize base_51_carry)
          As base_51_carry_correct.
   Proof. Time solve_rcarry machine_wordsize. Time Qed.
   Derive base_51_add
-         SuchThat (radd_correctT n s c base_51_add)
+         SuchThat (radd_correctT n s c machine_wordsize base_51_add)
          As base_51_add_correct.
   Proof. Time solve_radd machine_wordsize. Time Qed.
   Derive base_51_sub
-         SuchThat (rsub_correctT n s c base_51_sub)
+         SuchThat (rsub_correctT n s c machine_wordsize base_51_sub)
          As base_51_sub_correct.
   Proof. Time solve_rsub machine_wordsize. Time Qed.
   Derive base_51_opp
-         SuchThat (ropp_correctT n s c base_51_opp)
+         SuchThat (ropp_correctT n s c machine_wordsize base_51_opp)
          As base_51_opp_correct.
   Proof. Time solve_ropp machine_wordsize. Time Qed.
   Derive base_51_encode
-         SuchThat (rencode_correctT n s c base_51_encode)
+         SuchThat (rencode_correctT n s c machine_wordsize base_51_encode)
          As base_51_encode_correct.
   Proof. Time solve_rencode machine_wordsize. Time Qed.
   Derive base_51_zero
-         SuchThat (rzero_correctT n s c base_51_zero)
+         SuchThat (rzero_correctT n s c machine_wordsize base_51_zero)
          As base_51_zero_correct.
   Proof. Time solve_rzero machine_wordsize. Time Qed.
   Derive base_51_one
-         SuchThat (rone_correctT n s c base_51_one)
+         SuchThat (rone_correctT n s c machine_wordsize base_51_one)
          As base_51_one_correct.
   Proof. Time solve_rone machine_wordsize. Time Qed.
   Lemma base_51_curve_good
